CoqOfRust/alloc/str.v
@@ -7719,7 +7719,7 @@ Module str.
                 (Ty.path "array")
                 [ Value.Integer IntegerKind.Usize 16 ]
                 [ Ty.path "bool" ] :=
-            repeat (| Value.Bool false, Value.Integer IntegerKind.Usize 16 |) in
+            repeat (Value.Bool false) (Value.Integer IntegerKind.Usize 16) in
           let~ _ : Ty.tuple [] :=
             M.read (|
               M.loop (|
