CoqOfRust/alloc/string.v
@@ -5508,10 +5508,9 @@ Module string.
                                               M.borrow (|
                                                 Pointer.Kind.MutRef,
                                                 M.alloc (|
-                                                  repeat (|
-                                                    Value.Integer IntegerKind.U8 0,
-                                                    Value.Integer IntegerKind.Usize 4
-                                                  |)
+                                                  repeat
+                                                    (Value.Integer IntegerKind.U8 0)
+                                                    (Value.Integer IntegerKind.Usize 4)
                                                 |)
                                               |)
                                             |)
@@ -7550,7 +7549,7 @@ Module string.
               |) in
             let~ bits :
                 Ty.apply (Ty.path "array") [ Value.Integer IntegerKind.Usize 4 ] [ Ty.path "u8" ] :=
-              repeat (| Value.Integer IntegerKind.U8 0, Value.Integer IntegerKind.Usize 4 |) in
+              repeat (Value.Integer IntegerKind.U8 0) (Value.Integer IntegerKind.Usize 4) in
             let~ bits :
                 Ty.apply (Ty.path "&") [] [ Ty.apply (Ty.path "slice") [] [ Ty.path "u8" ] ] :=
               M.call_closure (|
@@ -14586,10 +14585,9 @@ Module string.
                       M.borrow (|
                         Pointer.Kind.MutRef,
                         M.alloc (|
-                          repeat (|
-                            Value.Integer IntegerKind.U8 0,
-                            Value.Integer IntegerKind.Usize 4
-                          |)
+                          repeat
+                            (Value.Integer IntegerKind.U8 0)
+                            (Value.Integer IntegerKind.Usize 4)
                         |)
                       |)
                     |)
