CoqOfRust/revm/revm_interpreter/instructions/system.v
@@ -5642,10 +5642,9 @@ Module instructions.
                               (Ty.path "array")
                               [ Value.Integer IntegerKind.Usize 32 ]
                               [ Ty.path "u8" ] :=
-                          repeat (|
-                            Value.Integer IntegerKind.U8 0,
-                            Value.Integer IntegerKind.Usize 32
-                          |) in
+                          repeat
+                            (Value.Integer IntegerKind.U8 0)
+                            (Value.Integer IntegerKind.Usize 32) in
                         let~ _ : Ty.tuple [] :=
                           M.read (|
                             M.match_operator (|
